Hoare.v
@@ -1,0 +1,89 @@
+Require Export Imp.
+
+Definition Assertion := state -> Prop. 
+
+  
+Definition as1 : Assertion := fun st => st X = 3.
+Definition as2 : Assertion := fun st => st X <= st Y.
+Definition as3 : Assertion :=
+  fun st => st X = 3 \/ st X <= st Y.
+Definition as4 : Assertion :=
+  fun st => st Z * st Z <= st X /\
+            ~ (((S (st Z)) * (S (st Z))) <= st X).
+Definition as5 : Assertion := fun st => True.
+Definition as6 : Assertion := fun st => False.
+
+
+Definition assert_implies (P Q : Assertion) : Prop :=
+  forall st, P st -> Q st.
+
+Notation "P ->> Q" :=
+  (assert_implies P Q) (at level 80) : hoare_spec_scope.
+Open Scope hoare_spec_scope.
+
+Notation "P <<->> Q" :=
+  (P ->> Q /\ Q ->> P) (at level 80) : hoare_spec_scope.
+
+Definition hoare_triple (P : Assertion) (c : com) (Q : Assertion) : Prop :=
+  forall st st',
+    c / st || st' ->
+    P st ->
+    Q st'.
+
+Notation "{{ P }} c {{ Q }}" :=
+  (hoare_triple P c Q) (at level 90, c at next level)
+  : hoare_spec_scope.
+
+(*
+
+   1) {{True}} c {{X = 5}}
+
+   2) {{X = m}} c {{X = m + 5)}}
+
+   3) {{X <= Y}} c {{Y <= X}}
+
+   4) {{True}} c {{False}}
+
+   5) {{X = m}} 
+      c
+      {{Y = real_fact m}}.
+
+   6) {{True}} 
+      c 
+      {{(Z * Z) <= m ∧ ~ (((S Z) * (S Z)) <= m)}} 
+*)
+
+(*
+
+   1) {{True}} X ::= 5 {{X = 5}}
+
+   2) {{X = 2}} X ::= X + 1 {{X = 3}}
+
+   3) {{True}} X ::= 5; Y ::= 0 {{X = 5}}
+
+   4) {{X = 2 ∧ X = 3}} X ::= 5 {{X = 0}}
+
+   5) {{True}} SKIP {{False}}
+
+   6) {{False}} SKIP {{True}}
+
+   7) {{True}} WHILE True DO SKIP END {{False}}
+
+   8) {{X = 0}}
+      WHILE X == 0 DO X ::= X + 1 END
+      {{X = 1}}
+
+   9) {{X = 1}}
+      WHILE X <> 0 DO X ::= X + 1 END
+      {{X = 100}}
+*)
+
+Theorem ex_loop_quodlibet : forall P Q, hoare_triple P loop Q.
+  intros p q.
+  unfold hoare_triple.
+  intros.
+  apply ex_falso_quodlibet.
+  apply loop_doesnt_stop with st.
+  exists st'.
+  assumption.
+Qed. 
